theories/Props/Freshness.v
@@ -1,5 +1,10 @@
-From Reactive Require Import Base.
+Set Default Goal Selector "!".
+
+From Reactive.Props Require Import Identifier.
 From Stdlib.Arith Require Import PeanoNat.
+From Stdlib Require Import List.
+
+Definition freshness {A} (seed: ident) (vars: list (ident * A)) := forall n, ~In (Nat.iter n next_ident seed) (map fst vars).
 
 Lemma freshness_fusion {A} {seed: ident} {vars1 vars2: list (ident * A)}:
   freshness seed vars1 -> freshness seed vars2 -> freshness seed (vars1 ++ vars2).
@@ -14,7 +19,7 @@ Proof.
 Qed.
 
 Lemma freshness_later {A} {seed1 seed2: ident} {n: nat} {vars: list (ident * A)}:
-  seed2 = iter n next_ident seed1 -> freshness seed1 vars -> freshness seed2 vars.
+  seed2 = Nat.iter n next_ident seed1 -> freshness seed1 vars -> freshness seed2 vars.
 Proof.
   intros fresh1 isiter.
   intro m.
@@ -25,7 +30,7 @@ Proof.
 Qed.
 
 Lemma freshness_later_e {A} {seed1 seed2: ident} {vars: list (ident * A)}:
-  (exists n, seed2 = iter n next_ident seed1) -> freshness seed1 vars -> freshness seed2 vars.
+  (exists n, seed2 = Nat.iter n next_ident seed1) -> freshness seed1 vars -> freshness seed2 vars.
 Proof.
   intros [n isiter].
   apply (freshness_later isiter).
