theories/Languages/Semantics.v
@@ -1,0 +1,136 @@
+Set Default Goal Selector "!".
+
+From Stdlib Require Import Nat.
+From Reactive.Props Require Import Identifier Sigma.
+
+Inductive type : Set :=
+  | TVoid
+  | TBool
+  | TInt
+.
+
+Definition binder := prod ident type.
+Definition binder_ty (b : binder) : type := snd b.
+
+Lemma type_dec (x y: type): {x = y} + {x <> y}.
+Proof.
+  destruct x, y; try solve [left; reflexivity]; right; discriminate.
+Defined.
+
+Lemma binder_dec (x y: binder) : {x = y} + {x <> y}.
+Proof.
+  destruct x as [i1 ty1], y as [i2 ty2].
+  
+  pose proof (PeanoNat.Nat.eq_dec i1 i2).
+  destruct H.
+  2: {
+    right.
+    injection as eqi _.
+    contradiction.
+  }
+
+  destruct (type_dec ty1 ty2).
+  2: {
+    right.
+    injection as _ eqt.
+    contradiction.
+  }
+
+  left.
+  f_equal.
+  all: assumption.
+Defined.
+
+Definition sig2T_eq_type := @sig2T_eq _ type_dec.
+Arguments sig2T_eq_type {_ _ _ _}.
+
+Lemma type_dec_same : forall ty, type_dec ty ty = left eq_refl.
+Proof using.
+  intros ty.
+  destruct (type_dec ty ty) as [ e | n ]; [ | contradiction (n eq_refl) ].
+  f_equal.
+  apply Eqdep_dec.UIP_dec.
+  exact type_dec.
+Qed.
+
+Lemma forall_type_dec : forall (P : type -> Prop), (forall ty, {P ty} + {~P ty}) -> {forall ty, P ty} + {exists ty, ~ P ty}.
+Proof using.
+  intros P dec.
+  destruct (dec TVoid) as [Pvoid | nP]; [|right; exact (ex_intro (fun ty => ~ P ty) _ nP)].
+  destruct (dec TBool) as [Pbool | nP]; [|right; exact (ex_intro (fun ty => ~ P ty) _ nP)].
+  destruct (dec TInt)  as [Pint  | nP]; [|right; exact (ex_intro (fun ty => ~ P ty) _ nP)].
+  left; intros []; assumption.
+Defined.
+
+Definition type_eqb (x y: type): bool :=
+  match x, y with
+    | TVoid, TVoid => true
+    | TBool, TBool => true
+    | TInt, TInt => true
+    | _, _ => false
+  end.
+
+Lemma type_eqb_eq (x y: type):
+  type_eqb x y = true <-> x = y.
+Proof.
+  destruct x, y.
+  all: firstorder.
+  all: discriminate.
+Qed.
+
+Lemma type_eqb_refl (t: type):
+  type_eqb t t = true.
+Proof.
+  destruct t; reflexivity.
+Qed.
+
+Definition binder_eqb (x y: binder): bool :=
+  andb (fst x =? fst y) (type_eqb (snd x) (snd y)).
+
+  Lemma binder_eqb_refl (b: binder):
+  binder_eqb b b = true.
+Proof.
+  destruct b as (i, t).
+  apply andb_true_intro.
+  split.
+  - apply PeanoNat.Nat.eqb_refl.
+  - apply type_eqb_refl.
+Qed.
+
+Lemma binder_eqb_to_eq (x y : binder): binder_eqb x y = true -> x = y.
+Proof.
+  unfold binder_eqb, andb.
+  destruct (fst x =? fst y) eqn:Heq; [| discriminate ].
+
+  rewrite PeanoNat.Nat.eqb_eq in Heq.
+  destruct x, y; simpl in Heq |- *.
+  rewrite Heq.
+
+  intros H.
+  now destruct t, t0.
+Qed.
+
+Inductive const : type -> Set :=
+  | CVoid: const TVoid
+  | CBool: bool -> const TBool
+  | CInt: nat -> const TInt
+.
+Lemma const_inv {ty} (x: const ty) :
+  {eq : ty = _ & {b : bool | x = eq_rect _ const (CBool b) _ (eq_sym eq)}} +
+  {eq : ty = _ & {n : nat | x = eq_rect _ const (CInt n) _ (eq_sym eq)}} +
+  {exists (eq : ty = _), x = eq_rect _ const CVoid _ (eq_sym eq)}.
+Proof using.
+  destruct x as [|b|n]; [right|left; left|left; right]; exists eq_refl; [|exists b|exists n]; exact eq_refl.
+Defined.
+
+Lemma const_dec {ty} (x y: const ty) : {x = y} + {x <> y}.
+Proof.
+  destruct x as [ | b | n ].
+  all: destruct (const_inv y) as [[[eq' [b' ->]]|[eq' [n' ->]]]|H].
+  all: try discriminate; try solve [right; destruct H as [f _]; discriminate f].
+  1: left; destruct H as [eq' ->].
+  2: destruct (Bool.bool_dec b b') as [eq|ne]; [left|right].
+  4: destruct (PeanoNat.Nat.eq_dec n n') as [eq|ne]; [left|right].
+  all: rewrite !(Eqdep_dec.UIP_dec type_dec _ eq_refl); cbn; try intros [=f]; auto.
+  exact (f_equal _ eq).
+Defined.
