theories/Props/Forall.v
@@ -1,0 +1,8 @@
+Set Default Goal Selector "!".
+
+From Stdlib Require Import List.
+
+Lemma Forall_univ : forall [A] (P : A -> Prop), (forall x, P x) -> forall l, Forall P l.
+Proof using.
+  intros A P HP l; induction l as [|hd tl IH]; constructor; [exact (HP _)|exact IH].
+Qed.
