theories/Props/Axioms.v
@@ -1,0 +1,5 @@
+Set Default Goal Selector "!".
+
+Axiom ProofIrrelevance: forall (P: Prop) (p q: P), p = q.
+
+Axiom ABORT_FIXME : forall A : Type, unit -> A.
